Add MP+dmbs to UMPromising tests

ArchSemArm/tests/UMPromisingTest.v
@@ -56,9 +56,9 @@ Definition check_regs (reg : register_bitvector_64) (regs : registerMap)
     if reg_lookup reg regs is Some r0 then
       Ok (bv_unsigned r0)
     else
-      Error "R0 not in the thread state".
+      Error ((pretty (GReg reg)) +:+ " not in the thread state").
 
-Definition r_extract {n} (reg : register_bitvector_64) (tid : fin n)
+Definition reg_extract {n} (reg : register_bitvector_64) (tid : fin n)
     (a : Model.Res.t ∅ n) : result string Z :=
   match a with
   | Model.Res.FinalState fs =>
@@ -67,6 +67,19 @@ Definition r_extract {n} (reg : register_bitvector_64) (tid : fin n)
   | Model.Res.Error s => Error s
   | Model.Res.Unspecified e => match e with end
   end.
+
+Definition regs_extract {n} (regs : list (fin n * register_bitvector_64))
+  (a : Model.Res.t ∅ n) : result string (list Z) :=
+  match a with
+  | Model.Res.FinalState fs =>
+      for (tid, reg) in regs do
+        let regmap : registerMap := fs.(MState.regs) !!! tid in
+        check_regs reg regmap
+      end
+  | Model.Res.Error s => Error s
+  | Model.Res.Unspecified e => match e with end
+  end.
+
 
 (** We test against the sail-tiny-arm semantic, with non-determinism enabled *)
 Definition arm_sem := sail_tiny_arm_sem true.
@@ -101,7 +114,7 @@ Module EOR.
 
   Definition test_results := UMPromising_cert_c arm_sem fuel n_threads initState.
 
-  Goal r_extract R0 0%fin <$> test_results = Listset [Ok 0x110%Z].
+  Goal reg_extract R0 0%fin <$> test_results = Listset [Ok 0x110%Z].
     vm_compute (_ <$> _).
     reflexivity.
   Qed.
@@ -135,7 +148,7 @@ Module LDR. (* LDR X0, [X1, X0] at 0x500, loading from 0x1000 *)
 
   Definition test_results := UMPromising_cert_c arm_sem fuel n_threads initState.
 
-  Goal r_extract R0 0%fin <$> test_results = Listset [Ok 0x2a%Z].
+  Goal reg_extract R0 0%fin <$> test_results = Listset [Ok 0x2a%Z].
     vm_compute (_ <$> _).
     reflexivity.
   Qed.
@@ -171,7 +184,7 @@ Module STRLDR. (* STR X2, [X1, X0]; LDR X0, [X1, X0] at 0x500, using address 0x1
 
   Definition test_results := UMPromising_cert_c arm_sem fuel n_threads initState.
 
-  Goal r_extract R0 0%fin <$> test_results ≡ Listset [Ok 0x2a%Z].
+  Goal reg_extract R0 0%fin <$> test_results ≡ Listset [Ok 0x2a%Z].
     vm_compute (_ <$> _).
     set_solver.
   Qed.
@@ -236,14 +249,80 @@ Module MP.
   Definition test_results :=
     UMPromising_cert_c arm_sem fuel n_threads initState.
 
-  Definition test_tid : fin n_threads := 1%fin.
-  Definition test_reg := R2.
-  Definition test_out : listset (result string Z) :=
-    Listset [Ok 0x2a%Z; Ok 0x0%Z].
-
-  Goal test_out ≡ (r_extract test_reg test_tid <$> test_results).
-    vm_compute (_ <$> _).
-    unfold test_out.
-    set_solver.
+  Goal elements (regs_extract [(1%fin, R5); (1%fin, R2)] <$> test_results) ≡ₚ
+    [Ok [0x0%Z;0x2a%Z]; Ok [0x0%Z;0x0%Z]; Ok [0x1%Z; 0x2a%Z]; Ok [0x1%Z; 0x0%Z]].
+  Proof.
+    vm_compute (elements _).
+    apply NoDup_Permutation; try solve_NoDup; set_solver.
   Qed.
 End MP.
+
+Module MPDMBS.
+  (* A classic MP litmus test
+     Thread 1: STR X2, [X1, X0]; DMB SY; STR X5, [X4, X3]
+     Thread 2: LDR X5, [X4, X3]; DMB SY; LDR X2, [X1, X0]
+
+     Expected outcome of R2 at Thread 2: only 0x2a *)
+
+  Definition init_reg_t1 : registerMap :=
+    ∅
+    |> reg_insert _PC 0x500
+    |> reg_insert R0 0x1000
+    |> reg_insert R1 0x100
+    |> reg_insert R3 0x1000
+    |> reg_insert R4 0x200
+    |> reg_insert R2 0x2a
+    |> reg_insert R5 0x1.
+
+  Definition init_reg_t2 : registerMap :=
+    ∅
+    |> reg_insert _PC 0x600
+    |> reg_insert R0 0x1000
+    |> reg_insert R1 0x100
+    |> reg_insert R3 0x1000
+    |> reg_insert R4 0x200
+    |> reg_insert R2 0x0
+    |> reg_insert R5 0x0.
+
+  Definition init_mem : memoryMap :=
+    ∅
+    (* Thread 1 @ 0x500 *)
+    |> mem_insert 0x500 4 0xf8206822  (* STR X2, [X1, X0] *)
+    |> mem_insert 0x504 4 0xd5033fbf  (* DMB SY *)
+    |> mem_insert 0x508 4 0xf8236885  (* STR X5, [X4, X3] *)
+    (* Thread 2 @ 0x600 *)
+    |> mem_insert 0x600 4 0xf8636885  (* LDR X5, [X4, X3] *)
+    |> mem_insert 0x604 4 0xd5033fbf  (* DMB SY *)
+    |> mem_insert 0x608 4 0xf8606822  (* LDR X2, [X1, X0] *)
+    (* Backing memory so the addresses exist *)
+    |> mem_insert 0x1100 8 0x0
+    |> mem_insert 0x1200 8 0x0.
+
+  Definition n_threads := 2%nat.
+
+  Definition terminate_at := [# Some (0x50c : bv 64); Some (0x60c : bv 64)].
+
+  (* Each thread’s PC must reach the end of its three instructions *)
+  Definition termCond : terminationCondition n_threads :=
+    (λ tid rm, reg_lookup _PC rm =? terminate_at !!! tid).
+
+  Definition initState :=
+    {| MState.state :=
+        {| MState.memory := init_mem;
+            MState.regs := [# init_reg_t1; init_reg_t2];
+            MState.address_space := PAS_NonSecure |};
+      MState.termCond := termCond |}.
+
+  Definition fuel := 8%nat.
+
+  Definition test_results :=
+    UMPromising_cert_c arm_sem fuel n_threads initState.
+
+  (** The test is fenced enough, the 0x1;0x0 outcome is impossible*)
+  Goal elements (regs_extract [(1%fin, R5); (1%fin, R2)] <$> test_results) ≡ₚ
+    [Ok [0x0%Z;0x2a%Z]; Ok [0x0%Z;0x0%Z]; Ok [0x1%Z; 0x2a%Z]].
+  Proof.
+    vm_compute (elements _).
+    apply NoDup_Permutation; try solve_NoDup; set_solver.
+  Qed.
+End MPDMBS.
